Weidenbach_Book/Array_UInt.thy
@@ -6,6 +6,17 @@ begin
 definition nth_aa_u where
   \<open>nth_aa_u x L L' =  nth_aa x (nat_of_uint32 L) L'\<close>
 
+definition nth_aa' where
+  \<open>nth_aa' xs i j = do {
+      x \<leftarrow> Array.nth' xs i;
+      y \<leftarrow> arl_get x j;
+      return y}\<close>
+
+lemma nth_aa_u[code]:
+  \<open>nth_aa_u x L L' =  nth_aa' x (integer_of_uint32 L) L'\<close>
+  unfolding nth_aa_u_def nth_aa'_def nth_aa_def Array.nth'_def nat_of_uint32_code
+  by auto
+
 lemma nth_aa_uint_hnr[sepref_fr_rules]:
   assumes \<open>CONSTRAINT is_pure R\<close>
   shows
@@ -38,5 +49,84 @@ lemma array_replicate_custom_hnr_u[sepref_fr_rules]:
   using array_replicate_custom_hnr[of A]
   unfolding hfref_def
   by (sep_auto simp: uint32_nat_assn_nat_assn_nat_of_uint32)
+
+
+definition append_el_aa_u' :: "('a::{default,heap} array_list) array \<Rightarrow>
+  uint32 \<Rightarrow> 'a \<Rightarrow> ('a array_list) array Heap"where
+"append_el_aa_u' \<equiv> \<lambda>a i x.
+   Array.nth' a (integer_of_uint32 i) \<bind>
+   (\<lambda>j. arl_append j x \<bind>
+        (\<lambda>a'. Array.upd' a (integer_of_uint32 i) a' \<bind> (\<lambda>_. return a)))"
+
+lemma append_el_aa_append_el_aa_u':
+  \<open>append_el_aa xs (nat_of_uint32 i) j = append_el_aa_u' xs i j\<close>
+  unfolding append_el_aa_def append_el_aa_u'_def Array.nth'_def nat_of_uint32_code  Array.upd'_def
+  by (auto simp add: upd'_def upd_return max_def)
+
+
+lemma append_aa_hnr_u:
+  fixes R ::  \<open>'a \<Rightarrow> 'b :: {heap, default} \<Rightarrow> assn\<close>
+  assumes p: \<open>is_pure R\<close>
+  shows
+    \<open>(uncurry2 (\<lambda>xs i. append_el_aa xs (nat_of_uint32 i)), uncurry2 (RETURN \<circ>\<circ>\<circ> (\<lambda>xs i. append_ll xs (nat_of_uint32 i)))) \<in>
+     [\<lambda>((l,i),x). nat_of_uint32 i < length l]\<^sub>a (arrayO_assn (arl_assn R))\<^sup>d *\<^sub>a uint32_assn\<^sup>k *\<^sub>a R\<^sup>k \<rightarrow> (arrayO_assn (arl_assn R))\<close>
+proof -
+  obtain R' where R: \<open>the_pure R = R'\<close> and R': \<open>R = pure R'\<close>
+    using p by fastforce
+  have [simp]: \<open>(\<exists>\<^sub>Ax. arrayO_assn (arl_assn R) a ai * R x r * true * \<up> (x = a ! ba ! b)) =
+     (arrayO_assn (arl_assn R) a ai * R (a ! ba ! b) r * true)\<close> for a ai ba b r
+    by (auto simp: ex_assn_def)
+  show ?thesis -- \<open>TODO tune proof\<close>
+    apply sepref_to_hoare
+    apply (sep_auto simp: append_el_aa_def uint32_nat_rel_def br_def)
+     apply (simp add: arrayO_except_assn_def)
+     apply (rule sep_auto_is_stupid[OF p])
+    apply (sep_auto simp: array_assn_def is_array_def append_ll_def)
+    apply (simp add: arrayO_except_assn_array0[symmetric] arrayO_except_assn_def)
+    apply (subst_tac (2) i = \<open>nat_of_uint32 ba\<close> in heap_list_all_nth_remove1)
+     apply (solves \<open>simp\<close>)
+    apply (simp add: array_assn_def is_array_def)
+    apply (rule_tac x=\<open>p[nat_of_uint32 ba := (ab, bc)]\<close> in ent_ex_postI)
+    apply (subst_tac (2)xs'=a and ys'=p in heap_list_all_nth_cong)
+      apply (solves \<open>auto\<close>)[2]
+    apply (auto simp: star_aci)
+    done
+qed
+
+lemma append_el_aa_hnr'[sepref_fr_rules]:
+  shows \<open>(uncurry2 append_el_aa_u', uncurry2 (RETURN ooo append_ll))
+     \<in> [\<lambda>((W,L), j). L < length W]\<^sub>a
+        (arrayO_assn (arl_assn nat_assn))\<^sup>d *\<^sub>a uint32_nat_assn\<^sup>k *\<^sub>a nat_assn\<^sup>k \<rightarrow> (arrayO_assn (arl_assn nat_assn))\<close>
+    (is \<open>?a \<in> [?pre]\<^sub>a ?init \<rightarrow> ?post\<close>)
+  using append_aa_hnr_u[of nat_assn, simplified] unfolding hfref_def  uint32_nat_rel_def br_def pure_def
+   hn_refine_def append_el_aa_append_el_aa_u'
+  by auto
+
+
+definition nth_u where
+  \<open>nth_u xs n = nth xs (nat_of_uint32 n)\<close>
+
+definition nth_u_code where
+  \<open>nth_u_code xs n = Array.nth' xs (integer_of_uint32 n)\<close>
+
+lemma nth_u_hnr[sepref_fr_rules]:
+  assumes \<open>CONSTRAINT is_pure A\<close>
+  shows \<open>(uncurry nth_u_code, uncurry (RETURN oo nth_u)) \<in>
+     [\<lambda>(xs, n). nat_of_uint32 n < length xs]\<^sub>a (array_assn A)\<^sup>k *\<^sub>a uint32_assn\<^sup>k \<rightarrow> A\<close>
+proof -
+  obtain A' where
+    A: \<open>pure A' = A\<close>
+    using assms pure_the_pure by auto
+  then have A': \<open>the_pure A = A'\<close>
+    by auto
+  have [simp]: \<open>the_pure (\<lambda>a c. \<up> ((c, a) \<in> A')) = A'\<close>
+    unfolding pure_def[symmetric] by auto
+  show ?thesis
+    by sepref_to_hoare
+      (sep_auto simp: array_assn_def is_array_def
+       hr_comp_def list_rel_pres_length list_rel_update param_nth A' A[symmetric] ent_refl_true
+     list_rel_eq_listrel listrel_iff_nth pure_def  nth_u_code_def nth_u_def Array.nth'_def
+     nat_of_uint32_code)
+qed
 
 end
