Weidenbach_Book/CDCL_Two_Watched_Literals_List_Watched_Init_Trail_Code.thy
@@ -1805,7 +1805,7 @@ sepref_definition SAT_wl_code
   by sepref
 
 
-code_printing constant "shiftl :: nat \<Rightarrow> nat \<Rightarrow> nat" \<rightharpoonup>
+ code_printing constant "shiftl :: nat \<Rightarrow> nat \<Rightarrow> nat" \<rightharpoonup>
   (SML) "(nat'_of'_integer(IntInf.<</ (integer'_of'_nat((_)),/ Word.fromInt (integer'_of'_nat((_))))))"
 
 code_printing constant "shiftr :: nat \<Rightarrow> nat \<Rightarrow> nat" \<rightharpoonup>
